conversion of Message.thy to Isar format

src/HOL/Auth/Message.thy
@@ -7,22 +7,31 @@ Datatypes of agents and messages;
 Inductive relations "parts", "analz" and "synth"
 *)
 
-Message = Main +
+theory Message = Main
+files ("Message_lemmas.ML"):
+
+(*Eliminates a commonly-occurring expression*)
+lemma [simp] : "~ (ALL x. x~=y)"
+by blast
+
+(*Needed occasionally with spy_analz_tac, e.g. in analz_insert_Key_newK*)
+lemma [simp] : "A Un (B Un A) = B Un A"
+by blast
 
 types 
   key = nat
 
 consts
-  invKey :: key=>key
+  invKey :: "key=>key"
 
-rules
-  invKey "invKey (invKey K) = K"
+axioms
+  invKey [simp] : "invKey (invKey K) = K"
 
   (*The inverse of a symmetric key is itself;
     that of a public key is the private key and vice versa*)
 
 constdefs
-  isSymKey :: key=>bool
+  isSymKey :: "key=>bool"
   "isSymKey K == (invKey K = K)"
 
 datatype  (*We allow any number of friendly agents*)
@@ -43,7 +52,7 @@ syntax
   "@MTuple"      :: "['a, args] => 'a * 'b"       ("(2{|_,/ _|})")
 
 syntax (xsymbols)
-  "@MTuple"      :: "['a, args] => 'a * 'b"       ("(2\\<lbrace>_,/ _\\<rbrace>)")
+  "@MTuple"      :: "['a, args] => 'a * 'b"       ("(2\<lbrace>_,/ _\<rbrace>)")
 
 translations
   "{|x, y, z|}"   == "{|x, {|y, z|}|}"
@@ -52,50 +61,86 @@ translations
 
 constdefs
   (*Message Y, paired with a MAC computed with the help of X*)
-  HPair :: "[msg,msg]=>msg"                       ("(4Hash[_] /_)" [0, 1000])
+  HPair :: "[msg,msg] => msg"                       ("(4Hash[_] /_)" [0, 1000])
     "Hash[X] Y == {| Hash{|X,Y|}, Y|}"
 
   (*Keys useful to decrypt elements of a message set*)
-  keysFor :: msg set => key set
+  keysFor :: "msg set => key set"
   "keysFor H == invKey ` {K. EX X. Crypt K X : H}"
 
 (** Inductive definition of all "parts" of a message.  **)
 
-consts  parts   :: msg set => msg set
+consts  parts   :: "msg set => msg set"
 inductive "parts H"
-  intrs 
-    Inj     "X: H  ==>  X: parts H"
-    Fst     "{|X,Y|}   : parts H ==> X : parts H"
-    Snd     "{|X,Y|}   : parts H ==> Y : parts H"
-    Body    "Crypt K X : parts H ==> X : parts H"
+  intros 
+    Inj [intro]          : "X: H  ==> X : parts H"
+    Fst:     "{|X,Y|}   : parts H ==> X : parts H"
+    Snd:     "{|X,Y|}   : parts H ==> Y : parts H"
+    Body:    "Crypt K X : parts H ==> X : parts H"
+
+
+(*Monotonicity*)
+lemma parts_mono: "G<=H ==> parts(G) <= parts(H)"
+apply auto
+apply (erule parts.induct) 
+apply (auto dest: Fst Snd Body) 
+done
 
 
 (** Inductive definition of "analz" -- what can be broken down from a set of
     messages, including keys.  A form of downward closure.  Pairs can
     be taken apart; messages decrypted with known keys.  **)
 
-consts  analz   :: msg set => msg set
+consts  analz   :: "msg set => msg set"
 inductive "analz H"
-  intrs 
-    Inj     "X: H ==> X: analz H"
-    Fst     "{|X,Y|} : analz H ==> X : analz H"
-    Snd     "{|X,Y|} : analz H ==> Y : analz H"
-    Decrypt "[| Crypt K X : analz H; Key(invKey K): analz H |] ==> X : analz H"
+  intros 
+    Inj [intro,simp] :    "X: H ==> X: analz H"
+    Fst:     "{|X,Y|} : analz H ==> X : analz H"
+    Snd:     "{|X,Y|} : analz H ==> Y : analz H"
+    Decrypt [dest]: 
+             "[|Crypt K X : analz H; Key(invKey K): analz H|] ==> X : analz H"
 
+
+(*Monotonicity; Lemma 1 of Lowe's paper*)
+lemma analz_mono: "G<=H ==> analz(G) <= analz(H)"
+apply auto
+apply (erule analz.induct) 
+apply (auto dest: Fst Snd) 
+done
 
 (** Inductive definition of "synth" -- what can be built up from a set of
     messages.  A form of upward closure.  Pairs can be built, messages
     encrypted with known keys.  Agent names are public domain.
     Numbers can be guessed, but Nonces cannot be.  **)
 
-consts  synth   :: msg set => msg set
+consts  synth   :: "msg set => msg set"
 inductive "synth H"
-  intrs 
-    Inj     "X: H ==> X: synth H"
-    Agent   "Agent agt : synth H"
-    Number  "Number n  : synth H"
-    Hash    "X: synth H ==> Hash X : synth H"
-    MPair   "[| X: synth H;  Y: synth H |] ==> {|X,Y|} : synth H"
-    Crypt   "[| X: synth H;  Key(K) : H |] ==> Crypt K X : synth H"
+  intros 
+    Inj    [intro]:   "X: H ==> X: synth H"
+    Agent  [intro]:   "Agent agt : synth H"
+    Number [intro]:   "Number n  : synth H"
+    Hash   [intro]:   "X: synth H ==> Hash X : synth H"
+    MPair  [intro]:   "[|X: synth H;  Y: synth H|] ==> {|X,Y|} : synth H"
+    Crypt  [intro]:   "[|X: synth H;  Key(K) : H|] ==> Crypt K X : synth H"
+
+(*Monotonicity*)
+lemma synth_mono: "G<=H ==> synth(G) <= synth(H)"
+apply auto
+apply (erule synth.induct) 
+apply (auto dest: Fst Snd Body) 
+done
+
+(*NO Agent_synth, as any Agent name can be synthesized.  Ditto for Number*)
+inductive_cases Nonce_synth [elim!]: "Nonce n : synth H"
+inductive_cases Key_synth   [elim!]: "Key K : synth H"
+inductive_cases Hash_synth  [elim!]: "Hash X : synth H"
+inductive_cases MPair_synth [elim!]: "{|X,Y|} : synth H"
+inductive_cases Crypt_synth [elim!]: "Crypt K X : synth H"
+
+use "Message_lemmas.ML"
+
+method_setup spy_analz = {*
+    Method.no_args (Method.METHOD (fn facts => spy_analz_tac 1)) *}
+    "for proving the Fake case when analz is involved"
 
 end
